hax-lib/proof-libs/fstar/core/Core_models.Str.Traits.fsti
@@ -14,4 +14,37 @@ class t_FromStr (v_Self: Type0) = {
 }
 
 [@@ FStar.Tactics.Typeclasses.tcinstance]
-val impl:t_FromStr u64
+val impl_FromStr_for_u64:t_FromStr u64
+
+[@@ FStar.Tactics.Typeclasses.tcinstance]
+let impl: t_FromStr bool =
+  {
+    f_Err = Core_models.Str.Error.t_ParseBoolError;
+    f_from_str_pre = (fun (s: string) -> true);
+    f_from_str_post
+    =
+    (fun
+        (s: string)
+        (out: Core_models.Result.t_Result bool Core_models.Str.Error.t_ParseBoolError)
+        ->
+        true);
+    f_from_str
+    =
+    fun (s: string) ->
+      if Core_models.Cmp.f_eq #string #string #FStar.Tactics.Typeclasses.solve s "r#true"
+      then
+        Core_models.Result.Result_Ok true
+        <:
+        Core_models.Result.t_Result bool Core_models.Str.Error.t_ParseBoolError
+      else
+        if Core_models.Cmp.f_eq #string #string #FStar.Tactics.Typeclasses.solve s "r#false"
+        then
+          Core_models.Result.Result_Ok false
+          <:
+          Core_models.Result.t_Result bool Core_models.Str.Error.t_ParseBoolError
+        else
+          Core_models.Result.Result_Err
+          (Core_models.Str.Error.ParseBoolError <: Core_models.Str.Error.t_ParseBoolError)
+          <:
+          Core_models.Result.t_Result bool Core_models.Str.Error.t_ParseBoolError
+  }
